theories/common.v
@@ -130,6 +130,10 @@ Ltac remove_bools_options :=
     |- _ =>
     let Hoption := fresh "Hoption" in
     destruct exp eqn:Hoption; try by []
+  | H: (if ?exp then _ else _ ) = _
+    |- _ =>
+    let Hif := fresh "Hif" in
+    destruct exp eqn:Hif; try by []
   | H: is_true match ?exp with
        | Some _ => _
        | None => _
