theories/typing_inversion.v
@@ -26,9 +26,9 @@ Ltac resolve_compose Hcat Hempty IH :=
 Ltac resolve_weaken :=
   repeat eexists; repeat split; eauto => /=; subst; repeat rewrite -catA => //.
 
-Lemma BI_const_typing: forall C econst t1s t2s,
-    be_typing C [::BI_const econst] (Tf t1s t2s) ->
-    t2s = t1s ++ [::typeof econst].
+Lemma BI_const_num_typing: forall C econst t1s t2s,
+    be_typing C [::BI_const_num econst] (Tf t1s t2s) ->
+    t2s = t1s ++ [::T_num (typeof_num econst)].
 Proof.
   move => C econst t1s t2s HType.
   gen_ind_subst HType => //.
@@ -38,30 +38,42 @@ Proof.
     by eapply IHHType.
 Qed.
 
-Lemma BI_const2_typing: forall C econst1 econst2 t1s t2s,
-    be_typing C [::BI_const econst1; BI_const econst2] (Tf t1s t2s) ->
-    t2s = t1s ++ [::typeof econst1; typeof econst2].
+Lemma BI_const_vec_typing: forall C econst t1s t2s,
+    be_typing C [::BI_const_vec econst] (Tf t1s t2s) ->
+    t2s = t1s ++ [::T_vec (typeof_vec econst)].
+Proof.
+  move => C econst t1s t2s HType.
+  gen_ind_subst HType => //.
+  - by resolve_compose Econs HType1 IHHType2.
+  - rewrite - catA -cat_app.
+    f_equal.
+    by eapply IHHType.
+Qed.
+
+Lemma BI_const_num2_typing: forall C econst1 econst2 t1s t2s,
+    be_typing C [::BI_const_num econst1; BI_const_num econst2] (Tf t1s t2s) ->
+    t2s = t1s ++ [::T_num (typeof_num econst1); T_num (typeof_num econst2)].
 Proof.
   move => C econst1 econst2 t1s t2s HType.
   gen_ind_subst HType => //.
   - apply extract_list2 in H1; inversion H1; subst.
-    apply BI_const_typing in HType1; subst.
-    apply BI_const_typing in HType2; subst.
+    apply BI_const_num_typing in HType1; subst.
+    apply BI_const_num_typing in HType2; subst.
     by rewrite -catA.
   - rewrite - catA -cat_app.
     f_equal.
     by eapply IHHType.
 Qed.
 
-Lemma BI_const3_typing: forall C econst1 econst2 econst3 t1s t2s,
-    be_typing C [::BI_const econst1; BI_const econst2; BI_const econst3] (Tf t1s t2s) ->
-    t2s = t1s ++ [::typeof econst1; typeof econst2; typeof econst3].
+Lemma BI_const_num3_typing: forall C econst1 econst2 econst3 t1s t2s,
+    be_typing C [::BI_const_num econst1; BI_const_num econst2; BI_const_num econst3] (Tf t1s t2s) ->
+    t2s = t1s ++ [::T_num (typeof_num econst1); T_num (typeof_num econst2); T_num (typeof_num econst3)].
 Proof.
   move => C econst1 econst2 econst3 t1s t2s HType.
   gen_ind_subst HType => //.
   - apply extract_list3 in H1; inversion H1; subst.
-    apply BI_const2_typing in HType1; subst.
-    apply BI_const_typing in HType2; subst.
+    apply BI_const_num2_typing in HType1; subst.
+    apply BI_const_num_typing in HType2; subst.
     by rewrite -catA.
   - rewrite - catA -cat_app.
     f_equal.
@@ -70,7 +82,7 @@ Qed.
 
 Lemma Unop_typing: forall C t op t1s t2s,
     be_typing C [::BI_unop t op] (Tf t1s t2s) ->
-    t1s = t2s /\ exists ts, t1s = ts ++ [::t].
+    t1s = t2s /\ exists ts, t1s = ts ++ [::T_num t].
 Proof.
   move => C t op t1s t2s HType.
   gen_ind_subst HType.
@@ -83,7 +95,7 @@ Qed.
 
 Lemma Binop_typing: forall C t op t1s t2s,
     be_typing C [::BI_binop t op] (Tf t1s t2s) ->
-    t1s = t2s ++ [::t] /\ exists ts, t2s = ts ++ [::t].
+    t1s = t2s ++ [::T_num t] /\ exists ts, t2s = ts ++ [::T_num t].
 Proof.
   move => C t op t1s t2s HType.
   gen_ind_subst HType.
@@ -97,7 +109,7 @@ Qed.
 
 Lemma Testop_typing: forall C t op t1s t2s,
     be_typing C [::BI_testop t op] (Tf t1s t2s) ->
-    exists ts, t1s = ts ++ [::t] /\ t2s = ts ++ [::T_i32] /\ is_int_t t.
+    exists ts, t1s = ts ++ [::T_num t] /\ t2s = ts ++ [::T_num T_i32] /\ is_int_t t.
 Proof.
   move => C t op t1s t2s HType.
   gen_ind_subst HType.
@@ -110,7 +122,7 @@ Qed.
 
 Lemma Relop_typing: forall C t op t1s t2s,
     be_typing C [::BI_relop t op] (Tf t1s t2s) ->
-    exists ts, t1s = ts ++ [::t; t] /\ t2s = ts ++ [::T_i32].
+    exists ts, t1s = ts ++ [::T_num t; T_num t] /\ t2s = ts ++ [::T_num T_i32].
 Proof.
   move => C t op t1s t2s HType.
   gen_ind_subst HType.
@@ -123,7 +135,7 @@ Qed.
 
 Lemma Cvtop_typing: forall C t1 t2 op sx t1s t2s,
     be_typing C [::BI_cvtop t2 op t1 sx] (Tf t1s t2s) ->
-    exists ts, t1s = ts ++ [::t1] /\ t2s = ts ++ [::t2] /\ (op = CVO_reinterpret -> sx = None).
+    exists ts, t1s = ts ++ [::T_num t1] /\ t2s = ts ++ [::T_num t2] /\ (op = CVO_reinterpret -> sx = None).
 Proof.
   move => C t1 t2 op sx t1s t2s HType.
   gen_ind_subst HType; try by exists nil.
@@ -155,51 +167,58 @@ Proof.
     by resolve_weaken.
 Qed.
 
-Lemma Select_typing: forall C t1s t2s,
-    be_typing C [::BI_select] (Tf t1s t2s) ->
-    exists ts t, t1s = ts ++ [::t; t; T_i32] /\ t2s = ts ++ [::t].
+Lemma Select_typing: forall C t1s t2s ot,
+    be_typing C [::BI_select ot] (Tf t1s t2s) ->
+    exists ts t,
+      t1s = ts ++ [::t; t; T_num T_i32] /\
+        t2s = ts ++ [::t] /\
+        (ot = Some [::t] \/ is_numeric_type t).
 Proof.
-  move => C t1s t2s HType.
+  move => C t1s t2s ot HType.
   gen_ind_subst HType => //.
-  - by exists [::], t.
+  - exists [::], t; repeat split => //; by left.
+  - exists [::], t; repeat split => //; by right.
   - by resolve_compose Econs HType1 IHHType2.
-  - edestruct IHHType as [? [?[??]]] => //=; subst.
+  - edestruct IHHType as [? [?[?[??]]]] => //=; subst.
     repeat rewrite -cat_app; repeat rewrite catA.
     by repeat eexists.
 Qed.
 
-Lemma If_typing: forall C t1s t2s e1s e2s ts ts',
-    be_typing C [::BI_if (Tf t1s t2s) e1s e2s] (Tf ts ts') ->
-    exists ts0, ts = ts0 ++ t1s ++ [::T_i32] /\ ts' = ts0 ++ t2s /\
-                be_typing (upd_label C ([:: t2s] ++ tc_label C)) e1s (Tf t1s t2s) /\
-                be_typing (upd_label C ([:: t2s] ++ tc_label C)) e2s (Tf t1s t2s).
+Lemma If_typing: forall C tb e1s e2s ts ts',
+    be_typing C [::BI_if tb e1s e2s] (Tf ts ts') ->
+    exists ts0 ts1 ts2,
+      expand_t C tb = Some (Tf ts1 ts2) /\
+        ts = ts0 ++ ts1 ++ [::T_num T_i32] /\ ts' = ts0 ++ ts2 /\
+        be_typing (upd_label C ([:: ts2] ++ tc_labels C)) e1s (Tf ts1 ts2) /\
+        be_typing (upd_label C ([:: ts2] ++ tc_labels C)) e2s (Tf ts1 ts2).
 Proof.
-  move => C t1s t2s e1s e2s ts ts' HType.
+  move => C tb e1s e2s ts ts' HType.
   gen_ind_subst HType => //=.
-  - by exists [::].
+  - by exists [::], tn, ts'.
+  - by resolve_compose Econs HType1 IHHType2.
+  - edestruct IHHType as [ts0 [ts1 [ts2 [? [? [? [??]]]]]]] => //=; subst.
+    exists (ts ++ ts0), ts1, ts2.
+    split => //.
+    by resolve_weaken.
+Qed.
+
+Lemma Br_if_typing: forall C ts1 ts2 i,
+    be_typing C [::BI_br_if i] (Tf ts1 ts2) ->
+    exists ts ts', ts2 = ts ++ ts' /\ ts1 = ts2 ++ [::T_num T_i32] /\ lookup_N C.(tc_labels) i = Some ts'.
+Proof.
+  move => C ts1 ts2 i HType.
+  gen_ind_subst HType => //=.
+  - by exists nil, ts2.
   - by resolve_compose Econs HType1 IHHType2.
   - edestruct IHHType as [ts0 [? [? [? ?]]]] => //=; subst.
     exists (ts ++ ts0).
     by resolve_weaken.
 Qed.
 
-Lemma Br_if_typing: forall C ts1 ts2 i,
-    be_typing C [::BI_br_if i] (Tf ts1 ts2) ->
-    exists ts ts', ts2 = ts ++ ts' /\ ts1 = ts2 ++ [::T_i32] /\ i < length (tc_label C) /\ plop2 C i ts'.
-Proof.
-  move => C ts1 ts2 i HType.
-  gen_ind_subst HType => //=.
-  - by exists nil; eexists.
-  - by resolve_compose Econs HType1 IHHType2.
-  - edestruct IHHType as [ts0 [? [? [? [? ?]]]]] => //=; subst.
-    exists (ts ++ ts0).
-    by resolve_weaken.
-Qed.
-
 Lemma Br_table_typing: forall C ts1 ts2 ids i0,
     be_typing C [::BI_br_table ids i0] (Tf ts1 ts2) ->
-    exists ts1' ts, ts1 = ts1' ++ ts ++ [::T_i32] /\
-                         all (fun i => (i < length (tc_label C)) && (plop2 C i ts)) (ids ++ [::i0]).
+    exists ts1' ts, ts1 = ts1' ++ ts ++ [::T_num T_i32] /\
+                         List.Forall (fun i => lookup_N C.(tc_labels) i = Some ts) (ids ++ [::i0]).
 Proof.
   move => C ts1 ts2 ids i0 HType.
   gen_ind_subst HType.
@@ -211,81 +230,76 @@ Proof.
 Qed.
 
 Lemma Tee_local_typing: forall C i ts1 ts2,
-    be_typing C [::BI_tee_local i] (Tf ts1 ts2) ->
-    exists ts t, ts1 = ts2 /\ ts1 = ts ++ [::t] /\ i < length (tc_local C) /\
-                 List.nth_error (tc_local C) i = Some t.
+    be_typing C [::BI_local_tee i] (Tf ts1 ts2) ->
+    exists ts t, ts1 = ts2 /\ ts1 = ts ++ [::t] /\ lookup_N (tc_locals C) i = Some t.
 Proof.
   move => C i ts1 ts2 HType.
   gen_ind_subst HType.
   - by exists [::], t.
   - by resolve_compose Econs HType1 IHHType2.
-  - edestruct IHHType as [ts0 [t [? [? [??]]]]] => //=.
+  - edestruct IHHType as [ts0 [t [? [? ?]]]] => //=.
     exists (ts ++ ts0), t.
     by resolve_weaken.
 Qed.
 
 Lemma Get_local_typing: forall C i t1s t2s,
-    be_typing C [::BI_get_local i] (Tf t1s t2s) ->
-    exists t, List.nth_error (tc_local C) i = Some t /\
-    t2s = t1s ++ [::t] /\
-    i < length (tc_local C).
+    be_typing C [::BI_local_get i] (Tf t1s t2s) ->
+    exists t, lookup_N (tc_locals C) i = Some t /\
+    t2s = t1s ++ [::t].
 Proof.
   move => ???? HType.
   gen_ind_subst HType => //=.
   - by eexists; eauto.
   - by resolve_compose Econs HType1 IHHType2.
-  - edestruct IHHType as [?[?[??]]]; eauto => //=.
+  - edestruct IHHType as [?[??]]; eauto => //=.
     by resolve_weaken.
 Qed.
 
 Lemma Set_local_typing: forall C i t1s t2s,
-    be_typing C [::BI_set_local i] (Tf t1s t2s) ->
-    exists t, List.nth_error (tc_local C) i = Some t /\
-    t1s = t2s ++ [::t] /\
-    i < length (tc_local C).
+    be_typing C [::BI_local_set i] (Tf t1s t2s) ->
+    exists t, lookup_N (tc_locals C) i = Some t /\
+    t1s = t2s ++ [::t].
 Proof.
   move => ???? HType.
   gen_ind_subst HType => //=.
   - by eexists; eauto.
   - by resolve_compose Econs HType1 IHHType2.
-  - edestruct IHHType as [?[?[??]]]; eauto => //=.
+  - edestruct IHHType as [?[??]]; eauto => //=.
     by resolve_weaken.
 Qed.
   
 Lemma Get_global_typing: forall C i t1s t2s,
-    be_typing C [::BI_get_global i] (Tf t1s t2s) ->
-    exists t, option_map tg_t (List.nth_error (tc_global C) i) = Some t /\
-    t2s = t1s ++ [::t] /\
-    i < length (tc_global C).
+    be_typing C [::BI_global_get i] (Tf t1s t2s) ->
+    exists t, option_map tg_t (lookup_N (tc_globals C) i) = Some t /\
+    t2s = t1s ++ [::t].
 Proof.
   move => ???? HType.
   gen_ind_subst HType => //=.
   - by eexists; eauto.
   - by resolve_compose Econs HType1 IHHType2.
-  - edestruct IHHType as [?[?[??]]]; eauto => //=.
+  - edestruct IHHType as [?[??]]; eauto => //=.
     by resolve_weaken.
 Qed.
 
 Lemma Set_global_typing: forall C i t1s t2s,
-    be_typing C [::BI_set_global i] (Tf t1s t2s) ->
-    exists g t, List.nth_error (tc_global C) i = Some g /\
+    be_typing C [::BI_global_set i] (Tf t1s t2s) ->
+    exists g t, lookup_N (tc_globals C) i = Some g /\
     tg_t g = t /\
     is_mut g /\
-    t1s = t2s ++ [::t] /\
-    i < length (tc_global C).
+    t1s = t2s ++ [::t].
 Proof.
   intros ???? HType.
   gen_ind_subst HType => //=.
   - by do 2 eexists; eauto.
   - by resolve_compose Econs HType1 IHHType2.
-  - edestruct IHHType as [? [? [? [? [? [? ?]]]]]]; subst=> //=.
+  - edestruct IHHType as [? [? [? [? [? ?]]]]]; subst=> //=.
     by resolve_weaken.
 Qed.
 
 Lemma Load_typing: forall C t a off tp_sx t1s t2s,
     be_typing C [::BI_load t tp_sx a off] (Tf t1s t2s) ->
-    exists ts, t1s = ts ++ [::T_i32] /\ t2s = ts ++ [::t] /\
-                    tc_memory C <> nil /\
+    exists ts, t1s = ts ++ [::T_num T_i32] /\ t2s = ts ++ [::T_num t] /\
+                    tc_mems C <> nil /\
                     load_store_t_bounds a (option_projl tp_sx) t.
 Proof.
   intros ??????? HType.
@@ -299,8 +313,8 @@ Qed.
 
 Lemma Store_typing: forall C t a off tp t1s t2s,
     be_typing C [::BI_store t tp a off] (Tf t1s t2s) ->
-    t1s = t2s ++ [::T_i32; t] /\
-    tc_memory C <> nil /\
+    t1s = t2s ++ [::T_num T_i32; T_num t] /\
+    tc_mems C <> nil /\
     load_store_t_bounds a tp t.
 Proof.
   intros ??????? HType.
@@ -310,9 +324,9 @@ Proof.
     by resolve_weaken.
 Qed.
 
-Lemma Current_memory_typing: forall C t1s t2s,
-    be_typing C [::BI_current_memory] (Tf t1s t2s) ->
-    tc_memory C <> nil /\ t2s = t1s ++ [::T_i32].
+Lemma Memory_size_typing: forall C t1s t2s,
+    be_typing C [::BI_memory_size] (Tf t1s t2s) ->
+    tc_mems C <> nil /\ t2s = t1s ++ [::T_num T_i32].
 Proof.
   intros ??? HType.
   gen_ind_subst HType => //=.
@@ -321,9 +335,9 @@ Proof.
     by resolve_weaken.
 Qed.
 
-Lemma Grow_memory_typing: forall C t1s t2s,
-    be_typing C [::BI_grow_memory] (Tf t1s t2s) ->
-    exists ts, tc_memory C <> nil /\ t2s = t1s /\ t1s = ts ++ [::T_i32].
+Lemma Memory_grow_typing: forall C t1s t2s,
+    be_typing C [::BI_memory_grow] (Tf t1s t2s) ->
+    exists ts, tc_mems C <> nil /\ t2s = t1s /\ t1s = ts ++ [::T_num T_i32].
 Proof.
   intros ??? HType.
   gen_ind_subst HType => //=.
@@ -334,53 +348,51 @@ Proof.
     by resolve_weaken.
 Qed.
 
-Lemma Block_typing: forall C t1s t2s es tn tm,
-    be_typing C [::BI_block (Tf t1s t2s) es] (Tf tn tm) ->
-    exists ts, tn = ts ++ t1s /\ tm = ts ++ t2s /\
-               be_typing (upd_label C ([::t2s] ++ (tc_label C))) es (Tf t1s t2s).
+Lemma Block_typing: forall C tb es tn tm,
+    be_typing C [::BI_block tb es] (Tf tn tm) ->
+    exists ts ts1 ts2, expand_t C tb = Some (Tf ts1 ts2) /\ tn = ts ++ ts1 /\ tm = ts ++ ts2 /\
+               be_typing (upd_label C ([::ts2] ++ (tc_labels C))) es (Tf ts1 ts2).
 Proof.
-  intros ?????? HType.
+  intros ????? HType.
   gen_ind_subst HType => //=.
-  - by exists nil; eauto.
+  - by exists nil, tn0, tm0; eauto.
   - by resolve_compose Econs HType1 IHHType2.
-  - edestruct IHHType as [ts0 [? [? ?]]]; subst => //=.
+  - edestruct IHHType as [ts0 [ts1 [ts2 [? [? [? ?]]]]]]; subst => //=.
     exists (ts ++ ts0).
     by resolve_weaken.
 Qed.
 
-Lemma Loop_typing: forall C t1s t2s es tn tm,
-    be_typing C [::BI_loop (Tf t1s t2s) es] (Tf tn tm) ->
-    exists ts, tn = ts ++ t1s /\ tm = ts ++ t2s /\
-               be_typing (upd_label C ([::t1s] ++ (tc_label C))) es (Tf t1s t2s).
+Lemma Loop_typing: forall C tb es tn tm,
+    be_typing C [::BI_loop tb es] (Tf tn tm) ->
+    exists ts ts1 ts2, expand_t C tb = Some (Tf ts1 ts2) /\ tn = ts ++ ts1 /\ tm = ts ++ ts2 /\
+               be_typing (upd_label C ([::ts1] ++ (tc_labels C))) es (Tf ts1 ts2).
 Proof.
-  intros ?????? HType.
+  intros ????? HType.
   gen_ind_subst HType => //=.
-  - by exists nil; eauto.
+  - by exists nil, tn0, tm0; eauto.
   - by resolve_compose Econs HType1 IHHType2.
-  - edestruct IHHType as [ts0 [? [? ?]]]; subst => //=.
+  - edestruct IHHType as [ts0 [ts1 [ts2 [? [? [??]]]]]]; subst => //=.
     exists (ts ++ ts0).
     by resolve_weaken.
 Qed.
 
-Lemma Break_typing: forall n C t1s t2s,
+Lemma Branch_typing: forall n C t1s t2s,
     be_typing C [::BI_br n] (Tf t1s t2s) ->
-    exists ts ts0, n < size (tc_label C) /\
-               plop2 C n ts /\
+    exists ts ts0, lookup_N C.(tc_labels) n = Some ts /\
                t1s = ts0 ++ ts.
 Proof.
   intros ???? HType.
   gen_ind_subst HType => //=.
   - by do 2 eexists; eauto.
   - by resolve_compose Econs HType1 IHHType2.
-  - edestruct IHHType as [ts0 [ts' [? [??]]]]; subst => //=.
+  - edestruct IHHType as [ts0 [ts' [? ?]]]; subst => //=.
     exists ts0, (ts ++ ts').
     by resolve_weaken.
 Qed.
 
 Lemma Return_typing: forall C t1s t2s,
     be_typing C [::BI_return] (Tf t1s t2s) ->
-    exists ts ts', t1s = ts' ++ ts /\
-                   tc_return C = Some ts.
+    exists ts ts', t1s = ts' ++ ts /\ tc_return C = Some ts.
 Proof.
   intros ??? HType.
   gen_ind_subst HType => //=.
@@ -393,8 +405,8 @@ Qed.
 
 Lemma Call_typing: forall j C t1s t2s,
     be_typing C [::BI_call j] (Tf t1s t2s) ->
-    exists ts t1s' t2s', j < length (tc_func_t C) /\
-    List.nth_error (tc_func_t C) j = Some (Tf t1s' t2s') /\
+    exists ts t1s' t2s',
+    lookup_N (tc_funcs C) j = Some (Tf t1s' t2s') /\
                          t1s = ts ++ t1s' /\
                          t2s = ts ++ t2s'.
 Proof.
@@ -402,24 +414,25 @@ Proof.
   gen_ind_subst HType => //=.
   - by exists nil; do 2 eexists; eauto.
   - by resolve_compose Econs HType1 IHHType2.
-  - edestruct IHHType as [ts0 [ts1' [ts2' [?[?[??]]]]]]; subst => //=.
+  - edestruct IHHType as [ts0 [ts1' [ts2' [?[??]]]]]; subst => //=.
     exists (ts ++ ts0), ts1', ts2'.
     by resolve_weaken.
 Qed.
 
-Lemma Call_indirect_typing: forall i C t1s t2s,
-    be_typing C [::BI_call_indirect i] (Tf t1s t2s) ->
-    exists tn tm ts, tc_table C <> nil /\
-    i < length (tc_types_t C) /\
-    List.nth_error (tc_types_t C) i = Some (Tf tn tm) /\
-    t1s = ts ++ tn ++ [::T_i32] /\ t2s = ts ++ tm.
+Lemma Call_indirect_typing: forall x y C t1s t2s,
+    be_typing C [::BI_call_indirect x y] (Tf t1s t2s) ->
+    exists tn tm tabtype ts,
+      lookup_N (tc_tables C) x = Some tabtype /\
+        tt_elem_type tabtype = T_funcref /\
+        lookup_N (tc_types C) y = Some (Tf tn tm) /\
+        t1s = ts ++ tn ++ [::T_num T_i32] /\ t2s = ts ++ tm.
 Proof.
-  intros ???? HType.
+  intros ????? HType.
   gen_ind_subst HType => //=.
-  - by do 2 eexists; exists nil; eauto.
+  - by do 3 eexists; exists nil; eauto.
   - by resolve_compose Econs HType1 IHHType2.
-  - edestruct IHHType as [ts0 [ts1' [ts2' [?[?[?[??]]]]]]]; subst => //=.
-    exists ts0, ts1', (ts ++ ts2').
+  - edestruct IHHType as [ts0 [ts1' [tabt [ts2' [?[?[?[??]]]]]]]]; subst => //=.
+    exists ts0, ts1', tabt, (ts ++ ts2').
     by resolve_weaken.
 Qed.
 
@@ -441,7 +454,6 @@ Lemma be_composition_typing_single: forall C es1 e t1s t2s,
 Proof.
   move => C es1 e t1s t2s HType.
   gen_ind_subst HType; extract_listn; auto_prove_bet.
-  + by apply bet_block.
   + by destruct es1 => //=.
   + apply concat_cancel_last in Ecat as [-> ->].
     by exists t2s.
@@ -495,8 +507,9 @@ Proof.
   by eapply bet_composition'; eauto.
 Qed.
 
+(*
 Lemma Const_list_typing: forall C vs t1s t2s,
-    be_typing C (to_b_list (v_to_e_list vs)) (Tf t1s t2s) ->
+    be_typing C (v_to_b_list vs) (Tf t1s t2s) ->
     t2s = t1s ++ (map typeof vs).
 Proof.
   move => C vs.
@@ -521,6 +534,7 @@ Proof.
   eapply bet_composition'; eauto.
   by apply bet_weakening_empty_1.
 Qed.
+*)
 
 End Typing_inversion_be.
 
@@ -536,12 +550,14 @@ Ltac invert_be_typing:=
     extract_listn
   | H: be_typing _ [::] _ |- _ =>
     apply empty_typing in H; subst
-  | H: be_typing _ [:: BI_const _] _ |- _ =>
-    apply BI_const_typing in H; subst
-  | H: be_typing _ [:: BI_const _; BI_const _] _ |- _ =>
-    apply BI_const2_typing in H; subst
-  | H: be_typing _ [:: BI_const _; BI_const _; BI_const _] _ |- _ =>
-    apply BI_const3_typing in H; subst
+  | H: be_typing _ [:: BI_const_num _] _ |- _ =>
+    apply BI_const_num_typing in H; subst
+  | H: be_typing _ [:: BI_const_vec _] _ |- _ =>
+    apply BI_const_vec_typing in H; subst
+  | H: be_typing _ [:: BI_const_num _; BI_const_num _] _ |- _ =>
+    apply BI_const_num2_typing in H; subst
+  | H: be_typing _ [:: BI_const_num _; BI_const_num _; BI_const_num _] _ |- _ =>
+    apply BI_const_num3_typing in H; subst
   | H: be_typing _ [::BI_unop _ _] _ |- _ =>
     let ts := fresh "ts_unop" in
     let H1 := fresh "H1_unop" in
@@ -569,6 +585,8 @@ Ltac invert_be_typing:=
     let H2 := fresh "H2_cvtop" in
     let H3 := fresh "H3_cvtop" in
     apply Cvtop_typing in H; destruct H as [ts [H1 [H2 H3]]]; subst
+  | H: be_typing _ [::BI_nop] _ |- _ =>
+    apply Nop_typing in H; destruct H; subst
   | H: be_typing _ [::BI_drop] _ |- _ =>
     apply Drop_typing in H; destruct H; subst
   | H: be_typing _ [::BI_select] _ |- _ =>
@@ -576,63 +594,61 @@ Ltac invert_be_typing:=
     let t := fresh "t_select" in
     let H1 := fresh "H1_select" in
     let H2 := fresh "H2_select" in
-    apply Select_typing in H; destruct H as [ts [t [H1 H2]]]; subst
+    let H3 := fresh "H3_select" in
+    apply Select_typing in H; destruct H as [ts [t [H1 [H2 H3]]]]; subst
   | H: be_typing _ [::BI_if _ _ _] _ |- _ =>
     let ts := fresh "ts_if" in
+    let ts1 := fresh "ts1_if" in
+    let ts2 := fresh "ts2_if" in
+    let Hexpand := fresh "Hexpand_if" in
     let H1 := fresh "H1_if" in
     let H2 := fresh "H2_if" in
     let H3 := fresh "H3_if" in
     let H4 := fresh "H4_if" in
-    apply If_typing in H; destruct H as [ts [H1 [H2 [H3 H4]]]]; subst
+    apply If_typing in H; destruct H as [ts [ts1 [ts2 [Hexpand [H1 [H2 [H3 H4]]]]]]]; subst
   | H: be_typing _ [::BI_br_if _] _ |- _ =>
     let ts := fresh "ts_brif" in
     let ts' := fresh "ts'_brif" in
     let H1 := fresh "H1_brif" in
     let H2 := fresh "H2_brif" in
     let H3 := fresh "H3_brif" in
-    let H4 := fresh "H4_brif" in
-    apply Br_if_typing in H; destruct H as [ts [ts' [H1 [H2 [H3 H4]]]]]; subst
+    apply Br_if_typing in H; destruct H as [ts [ts' [H1 [H2 H3]]]]; subst
   | H: be_typing _ [::BI_br_table _ _] _ |- _ =>
     let ts := fresh "ts_brtable" in
     let ts' := fresh "ts'_brtable" in
     let H1 := fresh "H1_brtable" in
     let H2 := fresh "H2_brtable" in
     apply Br_table_typing in H; destruct H as [ts [ts' [H1 H2]]]; subst
-  | H: be_typing _ [::BI_tee_local _] _ |- _ =>
+  | H: be_typing _ [::BI_local_tee _] _ |- _ =>
     let ts := fresh "ts_teelocal" in
     let t := fresh "t_teelocal" in
     let H1 := fresh "H1_teelocal" in
     let H2 := fresh "H2_teelocal" in
     let H3 := fresh "H3_teelocal" in
-    let H4 := fresh "H4_teelocal" in
-    apply Tee_local_typing in H; destruct H as [ts [t [H1 [H2 [H3 H4]]]]]; subst
-  | H: be_typing _ [::BI_get_local _] _ |- _ =>
+    apply Tee_local_typing in H; destruct H as [ts [t [H1 [H2 H3]]]]; subst
+  | H: be_typing _ [::BI_local_get _] _ |- _ =>
     let ts := fresh "ts_getlocal" in
     let H1 := fresh "H1_getlocal" in
     let H2 := fresh "H2_getlocal" in
-    let H3 := fresh "H3_getlocal" in
-    apply Get_local_typing in H; destruct H as [ts [H1 [H2 H3]]]; subst
-  | H: be_typing _ [::BI_set_local _] _ |- _ =>
+    apply Get_local_typing in H; destruct H as [ts [H1 H2]]; subst
+  | H: be_typing _ [::BI_local_set _] _ |- _ =>
     let ts := fresh "ts_setlocal" in
     let H1 := fresh "H1_setlocal" in
     let H2 := fresh "H2_setlocal" in
-    let H3 := fresh "H3_setlocal" in
-    apply Set_local_typing in H; destruct H as [ts [H1 [H2 H3]]]; subst
-  | H: be_typing _ [::BI_get_global _] _ |- _ =>
+    apply Set_local_typing in H; destruct H as [ts [H1 H2]]; subst
+  | H: be_typing _ [::BI_global_get _] _ |- _ =>
     let ts := fresh "ts_getglobal" in
     let H1 := fresh "H1_getglobal" in
     let H2 := fresh "H2_getglobal" in
-    let H3 := fresh "H3_getglobal" in
-    apply Get_global_typing in H; destruct H as [ts [H1 [H2 H3]]]; subst
-  | H: be_typing _ [::BI_set_global _] _ |- _ =>
+    apply Get_global_typing in H; destruct H as [ts [H1 H2]]; subst
+  | H: be_typing _ [::BI_global_set _] _ |- _ =>
     let g := fresh "g_setglobal" in
     let t := fresh "t_setglobal" in
     let H1 := fresh "H1_setglobal" in
     let H2 := fresh "H2_setglobal" in
     let H3 := fresh "H3_setglobal" in
     let H4 := fresh "H4_setglobal" in
-    let H5 := fresh "H5_setglobal" in
-    apply Set_global_typing in H; destruct H as [g [t [H1 [H2 [H3 [H4 H5]]]]]]; subst
+    apply Set_global_typing in H; destruct H as [g [t [H1 [H2 [H3 H4]]]]]; subst
   | H: be_typing _ [::BI_load _ _ _ _] _ |- _ =>
     let ts := fresh "ts_load" in
     let H1 := fresh "H1_load" in
@@ -645,35 +661,38 @@ Ltac invert_be_typing:=
     let H2 := fresh "H2_store" in
     let H3 := fresh "H3_store" in
     apply Store_typing in H; destruct H as [H1 [H2 H3]]; subst
-  | H: be_typing _ [::BI_current_memory] _ |- _ =>
-    let H1 := fresh "H1_currentmemory" in
-    let H2 := fresh "H2_currentmemory" in
-    apply Current_memory_typing in H; destruct H as [H1 H2]; subst
-  | H: be_typing _ [::BI_grow_memory] _ |- _ =>
+  | H: be_typing _ [::BI_memory_size] _ |- _ =>
+    let H1 := fresh "H1_memorysize" in
+    let H2 := fresh "H2_memorysize" in
+    apply Memory_size_typing in H; destruct H as [H1 H2]; subst
+  | H: be_typing _ [::BI_memory_grow] _ |- _ =>
     let ts := fresh "ts_growmemory" in
     let H1 := fresh "H1_growmemory" in
     let H2 := fresh "H2_growmemory" in
     let H3 := fresh "H3_growmemory" in
-    apply Grow_memory_typing in H; destruct H as [ts [H1 [H2 H3]]]; subst
+    apply Memory_grow_typing in H; destruct H as [ts [H1 [H2 H3]]]; subst
   | H: be_typing _ [::BI_block _ _] _ |- _ =>
     let ts := fresh "ts_block" in
+    let ts1 := fresh "ts1_block" in
+    let ts2 := fresh "ts2_block" in
     let H1 := fresh "H1_block" in
     let H2 := fresh "H2_block" in
     let H3 := fresh "H3_block" in
-    apply Block_typing in H; destruct H as [ts [H1 [H2 H3]]]; subst
+    apply Block_typing in H; destruct H as [ts [ts1 [ts2 [Hexpand [H1 [H2 H3]]]]]]; subst
   | H: be_typing _ [::BI_loop _ _] _ |- _ =>
     let ts := fresh "ts_loop" in
+    let ts1 := fresh "ts1_loop" in
+    let ts2 := fresh "ts2_loop" in
     let H1 := fresh "H1_loop" in
     let H2 := fresh "H2_loop" in
     let H3 := fresh "H3_loop" in
-    apply Loop_typing in H; destruct H as [ts [H1 [H2 H3]]]; subst
+    apply Loop_typing in H; destruct H as [ts [ts1 [ts2 [Hexpand [H1 [H2 H3]]]]]]; subst
   | H: be_typing _ [::BI_br _] _ |- _ =>
     let ts := fresh "ts_br" in
     let ts0 := fresh "ts0_br" in
     let H1 := fresh "H1_br" in
     let H2 := fresh "H2_br" in
-    let H3 := fresh "H3_br" in
-    apply Break_typing in H; destruct H as [ts [ts0 [H1 [H2 H3]]]]; subst
+    apply Branch_typing in H; destruct H as [ts [ts0 [H1 H2]]]; subst
   | H: be_typing _ [::BI_return] _ |- _ =>
     let ts := fresh "ts_return" in
     let ts0 := fresh "ts0_return" in
@@ -687,20 +706,20 @@ Ltac invert_be_typing:=
     let H1 := fresh "H1_call" in
     let H2 := fresh "H2_call" in
     let H3 := fresh "H3_call" in
-    let H4 := fresh "H4_call" in
-    apply Call_typing in H; destruct H as [ts [ts1' [ts2' [H1 [H2 [H3 H4]]]]]]; subst
-  | H: be_typing _ (to_b_list (v_to_e_list _)) _ |- _ =>
-    apply Const_list_typing in H
-  | H: be_typing _ [::BI_call_indirect _] _ |- _ =>
+    apply Call_typing in H; destruct H as [ts [ts1' [ts2' [H1 [H2 H3]]]]]; subst
+ (* | H: be_typing _ (to_b_list (v_to_e_list _)) _ |- _ =>
+    apply Const_list_typing in H *)
+  | H: be_typing _ [::BI_call_indirect _ _] _ |- _ =>
     let ts := fresh "ts_callindirect" in
     let ts1' := fresh "ts1'_callindirect" in
+    let tabt := fresh "tabt_callindirect" in
     let ts2' := fresh "ts2'_callindirect" in
     let H1 := fresh "H1_callindirect" in
     let H2 := fresh "H2_callindirect" in
     let H3 := fresh "H3_callindirect" in
     let H4 := fresh "H4_callindirect" in
     let H5 := fresh "H5_callindirect" in
-    apply Call_indirect_typing in H; destruct H as [ts [ts1' [ts2' [H1 [H2 [H3 [H4 H5]]]]]]]; subst
+    apply Call_indirect_typing in H; destruct H as [ts [ts1' [tabt [ts2' [H1 [H2 [H3 [H4 H5]]]]]]]]; subst
   | H: be_typing _ (_ ++ _) _ |- _ =>
     let ts3 := fresh "ts3_comp" in
     let H1 := fresh "H1_comp" in
@@ -725,9 +744,9 @@ Section Typing_inversion_e.
 Variable host_function : eqType.
 
 Let store_record := store_record host_function.
-Let function_closure := function_closure host_function.
+Let funcinst := funcinst host_function.
 Let e_typing := @e_typing host_function.
-Let inst_typing : store_record -> instance -> t_context -> bool := @inst_typing _.
+Let inst_typing := @inst_typing host_function.
 
 Lemma e_composition_typing_single: forall s C es1 e t1s t2s,
     e_typing s C (es1 ++ [::e]) (Tf t1s t2s) ->
@@ -740,7 +759,7 @@ Proof.
     apply b_e_elim in H3. destruct H3. subst.
     rewrite to_b_list_concat in H.
     invert_be_typing.
-    apply basic_concat in H1. destruct H1.
+    apply basic_concat in H1. move/andP in H1. destruct H1.
     exists ts3_comp.
     by repeat split => //=; apply ety_a' => //=.
   - (* composition *)
@@ -755,10 +774,14 @@ Proof.
     repeat split => //=.
     + apply ety_a' => //. apply bet_weakening_empty_both. by apply bet_empty.
     + by apply ety_trap.
-  - (* Local *)
-    exists nil. repeat split => //=.
+  - (* Ref_extern *)
+    exists nil; repeat split => //.
     + by apply ety_a' => //; apply bet_empty.
-    + by apply ety_local.
+    + by econstructor.
+  - (* Ref *)
+    exists nil; repeat split => //.
+    + by apply ety_a' => //; apply bet_empty.
+    + by eapply ety_ref; eauto.
   - (* Invoke *)
     exists t1s. repeat split => //=.
     + apply ety_a' => //. apply bet_weakening_empty_both. by apply bet_empty.
@@ -767,6 +790,10 @@ Proof.
     exists nil. repeat split => //=.
     + by apply ety_a' => //; apply bet_empty.
     + by eapply ety_label; eauto.
+  - (* Frame *)
+    exists nil. repeat split => //=.
+    + by apply ety_a' => //; apply bet_empty.
+    + by apply ety_frame.
 Qed.
 
 Lemma e_composition_typing: forall s C es1 es2 t1s t2s,
@@ -812,7 +839,7 @@ Lemma Label_typing: forall s C n es0 es ts1 ts2,
     e_typing s C [::AI_label n es0 es] (Tf ts1 ts2) ->
     exists ts ts2', ts2 = ts1 ++ ts2' /\
                     e_typing s C es0 (Tf ts ts2') /\
-                    e_typing s (upd_label C ([::ts] ++ (tc_label C))) es (Tf [::] ts2') /\
+                    e_typing s (upd_label C ([::ts] ++ (tc_labels C))) es (Tf [::] ts2') /\
                     length ts = n.
 Proof.
   move => s C n es0 es ts1 ts2 HType.
@@ -832,10 +859,10 @@ Proof.
     by exists ts, ts2.
 Qed.
 
-Lemma Local_typing: forall s C n f es t1s t2s,
-    e_typing s C [::AI_local n f es] (Tf t1s t2s) ->
+Lemma Frame_typing: forall s C n f es t1s t2s,
+    e_typing s C [::AI_frame n f es] (Tf t1s t2s) ->
     exists ts, t2s = t1s ++ ts /\
-               s_typing s (Some ts) f es ts /\
+               thread_typing s (Some ts) (f, es) ts /\
                length ts = n.
 Proof.
   move => s C n f es ts1 ts2 HType.
@@ -853,7 +880,7 @@ Proof.
     exists ts2.
     repeat split => //=.
     by rewrite catA.
-  - (* ety_local *)
+  - (* ety_frame *)
     by exists ts2.
 Qed.
 
@@ -876,12 +903,12 @@ Ltac invert_e_typing :=
     let H4 := fresh "H4_label" in
     eapply Label_typing in H; eauto;
     destruct H as [ts [ts1 [H1 [H2 [H3 H4]]]]]; subst
-  | H: @e_typing _ _ _ [::AI_local _ _ _] _ |- _ =>
-    let ts := fresh "ts_local" in
-    let H1 := fresh "H1_local" in
-    let H2 := fresh "H2_local" in
-    let H3 := fresh "H3_local" in
-    eapply Local_typing in H; eauto;
+  | H: @e_typing _ _ _ [::AI_frame _ _ _] _ |- _ =>
+    let ts := fresh "ts_frame" in
+    let H1 := fresh "H1_frame" in
+    let H2 := fresh "H2_frame" in
+    let H3 := fresh "H3_frame" in
+    eapply Frame_typing in H; eauto;
     destruct H as [ts [H1 [H2 H3]]]; subst
   end.
 
@@ -890,9 +917,10 @@ Section Typing_inversion_e.
 Variable host_function : eqType.
 
 Let store_record := store_record host_function.
-Let function_closure := function_closure host_function.
+Let funcinst := funcinst host_function.
+Let funcinst_valid := @funcinst_valid host_function.
 Let e_typing := @e_typing host_function.
-Let inst_typing : store_record -> instance -> t_context -> bool := @inst_typing host_function.
+Let inst_typing := @inst_typing host_function.
 
 Ltac invert_e_typing' :=
   unfold e_typing in *; invert_e_typing.
@@ -901,23 +929,22 @@ Hint Transparent e_typing: core.
 
 Let host := host host_function.
 
-Variable host_instance : host.
+Variable host_moduleinst : host.
 
-Let host_state := host_state host_instance.
+Let host_state := host_state host_moduleinst.
 
 Let reduce : host_state -> store_record -> frame -> seq administrative_instruction ->
              host_state -> store_record -> frame -> seq administrative_instruction -> Prop
   := @reduce _ _.
 
-Let s_globals : store_record -> seq global := @s_globals _.
-Let s_mems : store_record -> seq memory := @s_mems _.
-Let functions_agree : seq function_closure -> nat -> function_type -> bool := @functions_agree _.
-Let cl_type : function_closure -> function_type := @cl_type _.
+Let s_globals : store_record -> seq globalinst := @s_globals _.
+Let s_mems : store_record -> seq meminst := @s_mems _.
+Let cl_type : funcinst -> function_type := @cl_type _.
 Let store_extension: store_record -> store_record -> Prop := @store_extension _.
 
 Lemma Invoke_func_typing: forall s C a t1s t2s,
     e_typing s C [::AI_invoke a] (Tf t1s t2s) ->
-    exists cl, List.nth_error s.(s_funcs) a = Some cl.
+    exists cl, lookup_N s.(s_funcs) a = Some cl.
 Proof.
   move => s C a t1s t2s HType.
   gen_ind_subst HType => //.
@@ -925,60 +952,34 @@ Proof.
   - apply extract_list1 in Econs. destruct Econs. subst.
     by eapply IHHType2 => //=.
   - by eapply IHHType => //=.
-  - by exists cl.
+  - unfold ext_func_typing in H; remove_bools_options.
+    by exists f.
 Qed.
 
-Lemma Invoke_func_native_typing: forall s i C a cl tn tm ts es t1s t2s,
-    e_typing s C [::AI_invoke a] (Tf t1s t2s) ->
-    List.nth_error s.(s_funcs) a = Some cl ->
-    cl = FC_func_native i (Tf tn tm) ts es ->
-    exists ts' C', t1s = ts' ++ tn /\ t2s = ts' ++ tm /\
-                inst_typing s i C' /\
-               be_typing (upd_local_label_return C' (tn ++ ts) ([::tm]) (Some tm)) es (Tf [::] tm).
+Lemma Invoke_func_native_typing: forall s C a ts1 ts2,
+    e_typing s C [::AI_invoke a] (Tf ts1 ts2) ->
+    exists ts tn tm,
+      ext_func_typing s a = Some (Tf tn tm) /\
+        ts1 = ts ++ tn /\
+        ts2 = ts ++ tm.
 Proof.
-  move => s i C a cl tn tm ts es t1s t2s HType HNth Hcl.
+  move => s C a ts1 ts2 HType.
   gen_ind_subst HType => //.
   - by destruct bes => //=.
   - apply extract_list1 in Econs. destruct Econs. subst.
     apply et_to_bet in HType1 => //=.
     apply empty_typing in HType1. subst.
     by eapply IHHType2 => //=.
-  - edestruct IHHType as [ts' [C' [? [??]]]]; eauto. subst.
-    exists (ts0 ++ ts'), C'.
+  - edestruct IHHType as [ts' [tn [tm [? [??]]]]]; eauto. subst.
+    exists (ts ++ ts'), tn, tm.
     by repeat split => //; rewrite catA.
-  - rewrite H in HNth.
-    injection HNth as ->.
-    inversion H0.
-    inversion H10; subst.
-    by exists [::], C.
-Qed.
-
-Lemma Invoke_func_host_typing: forall s C a cl h tn tm t1s t2s,
-    e_typing s C [::AI_invoke a] (Tf t1s t2s) ->
-    List.nth_error s.(s_funcs) a = Some cl ->
-    cl = FC_func_host (Tf tn tm) h ->
-    exists ts, t1s = ts ++ tn /\ t2s = ts ++ tm.
-Proof.
-  move => s C a cl h tn tm t1s t2s HType HNth Hcl.
-  gen_ind_subst HType => //.
-  - by destruct bes => //=.
-  - apply extract_list1 in Econs. destruct Econs. subst.
-    apply et_to_bet in HType1 => //=.
-    apply empty_typing in HType1. subst.
-    by eapply IHHType2 => //=.
-  - edestruct IHHType; eauto => //=.
-    exists (ts ++ x). destruct H. subst.
-    by split; repeat rewrite catA.
-  - rewrite H in HNth.
-    inversion HNth; subst; clear HNth.
-    inversion H0; subst.
-    by exists [::].
+  - exists nil; by repeat eexists.
 Qed.
 
 Lemma store_typed_cl_typed: forall s n f,
-    List.nth_error (s_funcs s) n = Some f ->
+    lookup_N (s_funcs s) n = Some f ->
     store_typing s ->
-    cl_typing s f (cl_type f).
+    funcinst_valid s f.
 Proof.
   move => s n f HN HST.
   unfold store_typing in HST.
@@ -986,40 +987,36 @@ Proof.
   remove_bools_options.
   simpl in HN.
   destruct HST.
-  (* arrow actually required to avoid ssreflect hijacking the rewrite tactic! *)
   rewrite -> List.Forall_forall in H.
   apply List.nth_error_In in HN.
-  apply H in HN. unfold cl_type_check_single in HN. destruct HN.
-  by inversion H1; subst.
+  by apply H in HN.
 Qed.
 
 (* inst_typing inversion *)
 Lemma inst_t_context_local_empty: forall s i C,
-    inst_typing s i C ->
-    tc_local C = [::].
+    inst_typing s i = Some C ->
+    tc_locals C = [::].
 Proof.
   move => s i C HInstType.
-  unfold inst_typing in HInstType.
+  unfold inst_typing, typing.inst_typing in HInstType.
   destruct i => //=.
-  destruct C => //=.
-  by destruct tc_local.
+  by remove_bools_options.
 Qed.
 
 Lemma inst_t_context_label_empty: forall s i C,
-    inst_typing s i C ->
-    tc_label C = [::].
+    inst_typing s i = Some C ->
+    tc_labels C = [::].
 Proof.
   move => s i C HInstType.
-  unfold inst_typing in HInstType.
+  unfold inst_typing, typing.inst_typing in HInstType.
   destruct i => //=.
-  destruct C => //=.
-  by destruct tc_local; destruct tc_label.
+  by remove_bools_options.
 Qed.
 
 Lemma global_type_reference: forall s i j C v t,
-    inst_typing s i C ->
+    inst_typing s i = Some C ->
     sglob_val s i j = Some v ->
-    option_map tg_t (List.nth_error (tc_global C) j) = Some t ->
+    option_map tg_t (lookup_N (tc_globals C) j) = Some t ->
     typeof v = t.
 Proof.
   move => s i j C v t HInstType Hvref Htref.
@@ -1032,7 +1029,7 @@ Proof.
   remove_bools_options.
   unfold inst_typing in HInstType.
   destruct i => //=. destruct C => //=.
-  destruct tc_local => //=. destruct tc_label => //=. destruct tc_return => //=.
+  destruct tc_locals => //=. destruct tc_labels => //=. destruct tc_return => //=.
   move/andP in HInstType. destruct HInstType.
   remove_bools_options.
   eapply all2_projection in H2; eauto.
@@ -1045,8 +1042,8 @@ Qed.
 
 Lemma func_context_store: forall s i C j x,
     inst_typing s i C ->
-    j < length (tc_func_t C) ->
-    List.nth_error (tc_func_t C) j = Some x ->
+    j < length (tc_funcs C) ->
+    List.nth_error (tc_funcs C) j = Some x ->
     exists a, List.nth_error i.(inst_funcs) j = Some a.
 Proof.
   move => s i C j x HIT HLength HN.
@@ -1054,7 +1051,7 @@ Proof.
   unfold sfunc_ind.
   unfold inst_typing, typing.inst_typing in HIT.
   destruct i => //=. destruct C => //=.
-  destruct tc_local => //=. destruct tc_label => //=. destruct tc_return => //=.
+  destruct tc_locals => //=. destruct tc_labels => //=. destruct tc_return => //=.
   remove_bools_options.
   remember H3 as H4. clear HeqH4.
   apply all2_size in H3.
@@ -1069,8 +1066,8 @@ Qed.
 
 Lemma glob_context_store: forall s i C j g,
     inst_typing s i C ->
-    j < length (tc_global C) ->
-    List.nth_error (tc_global C) j = Some g ->
+    j < length (tc_globals C) ->
+    List.nth_error (tc_globals C) j = Some g ->
     sglob s i j <> None.
 Proof.
   move => s i C j g HIT HLength HN.
@@ -1078,7 +1075,7 @@ Proof.
   unfold sglob_ind.
   unfold inst_typing, typing.inst_typing in HIT.
   destruct i => //=. destruct C => //=.
-  destruct tc_local => //=. destruct tc_label => //=. destruct tc_return => //=.
+  destruct tc_locals => //=. destruct tc_labels => //=. destruct tc_return => //=.
   remove_bools_options.
   remember H2 as H4. clear HeqH4.
   apply all2_size in H2.
@@ -1097,21 +1094,21 @@ Qed.
 
 Lemma mem_context_store: forall s i C,
     inst_typing s i C ->
-    tc_memory C <> [::] ->
+    tc_mems C <> [::] ->
     exists n, smem_ind s i = Some n /\
               List.nth_error (s_mems s) n <> None.
 Proof.
   move => s i C HIT HMemory.
   unfold inst_typing, typing.inst_typing in HIT.
   destruct i => //=. destruct C => //=.
-  destruct tc_local => //=. destruct tc_label => //=. destruct tc_return => //=.
+  destruct tc_locals => //=. destruct tc_labels => //=. destruct tc_return => //=.
   remove_bools_options.
   simpl in HMemory. unfold smem_ind. simpl.
   remember H0 as H4. clear HeqH4.
   apply all2_size in H0.
-  destruct inst_memory => //=; first by destruct tc_memory.
+  destruct inst_memory => //=; first by destruct tc_mems.
   exists m. split => //.
-  destruct tc_memory => //.
+  destruct tc_mems => //.
   simpl in H4.
   unfold memi_agree in H4.
   unfold s_mems.
@@ -1129,13 +1126,13 @@ Proof.
   unfold store_typing, tab_agree, tabcl_agree in HST.
   unfold stab_addr in HStab.
   destruct s => //=. destruct f => //=. destruct f_inst. destruct f_inst. destruct C => //=.
-  destruct tc_local => //=. destruct tc_label => //=. destruct tc_return => //=.
+  destruct tc_locals => //=. destruct tc_labels => //=. destruct tc_return => //=.
   remove_bools_options.
   simpl in *. destruct inst_tab0 => //=.
   unfold stab_index in HStab. unfold option_bind in HStab.
   remove_bools_options.
   subst. simpl in *.
-  destruct tc_table => //=.
+  destruct tc_tables => //=.
   remove_bools_options.
   destruct HST.
   destruct H5.
@@ -1176,7 +1173,7 @@ Ltac auto_basic :=
 end.
 
 Lemma Lfilled_break_typing: forall n m k (lh: lholed n) vs LI ts s C t2s tss,
-    e_typing s (upd_label C (tss ++ [::ts] ++ tc_label C)) LI (Tf [::] t2s) ->
+    e_typing s (upd_label C (tss ++ [::ts] ++ tc_labels C)) LI (Tf [::] t2s) ->
     const_list vs ->
     length ts = length vs ->
     lfill lh (vs ++ [::AI_basic (BI_br m)]) = LI ->
@@ -1257,8 +1254,8 @@ Proof.
     by eapply IHlh; eauto.
 Qed.
 
-Lemma Local_return_typing {k}: forall s C vs f LI tf (lh: lholed k),
-    e_typing s C [:: AI_local (length vs) f LI] tf ->
+Lemma Frame_return_typing {k}: forall s C vs f LI tf (lh: lholed k),
+    e_typing s C [:: AI_frame (length vs) f LI] tf ->
     const_list vs ->
     lfill lh (vs ++ [::AI_basic BI_return]) = LI ->
     e_typing s C vs tf.
